src/Prototype/Correctness.v
@@ -7,8 +7,8 @@ Open Scope fmap.
 Section System.
   Variables extIdx1 extIdx2: nat.
 
-  Local Definition IState := State SingleValueMsg ImplState.
-  Local Definition SState := State SingleValueMsg SpecState.
+  Local Definition IState := State SVMType SVM ImplState.
+  Local Definition SState := State SVMType SVM SpecState.
 
   Definition validValue (p c1 c2: ImplState) :=
     match impl_status p with
@@ -38,14 +38,14 @@ Section System.
   Defined.
 
   Theorem sim_simulates:
-    Simulates sim (impl extIdx1 extIdx2) (spec extIdx1 extIdx2).
+    Simulates svmT_dec svm_dec sim (impl extIdx1 extIdx2) (spec extIdx1 extIdx2).
   Proof.
     unfold Simulates; intros.
     
   Admitted.
 
   Theorem impl_refines_spec:
-    Refines (impl extIdx1 extIdx2) (spec extIdx1 extIdx2).
+    Refines svmT_dec svm_dec (impl extIdx1 extIdx2) (spec extIdx1 extIdx2).
   Proof.
     apply simulation_implies_refinement with (sim:= sim).
     - apply sim_simulates.
