src/Prototype/Transaction.v
@@ -2,41 +2,41 @@ Require Import Bool List String Peano_dec.
 Require Import FMap Language.
 
 Section System.
-  Context {MsgT StateT: Type}.
-  Context {MvalT: MsgT -> RqRs -> Type}.
+  Context {MsgT ValT StateT: Type}.
   Hypothesis (msgT_dec : forall m1 m2 : MsgT, {m1 = m2} + {m1 <> m2}).
+  Hypothesis (valT_dec : forall v1 v2 : ValT, {v1 = v2} + {v1 <> v2}).
 
   Local Notation isTrsPair := (isTrsPair msgT_dec).
 
   Definition CondT := StateT -> Prop.
   Definition condImp (c1 c2: CondT) := forall st, c1 st -> c2 st.
   Infix "-->" := condImp (at level 30).
-  Definition postOf (pmsg: PMsg MvalT StateT): CondT :=
+  Definition postOf (pmsg: PMsg MsgT ValT StateT): CondT :=
     fun post => forall pre mt, pmsg_postcond pmsg pre mt post.
 
   Definition Disjoint (c1 c2: CondT) := forall st, c1 st -> c2 st -> False.
   Infix "-*-" := Disjoint (at level 30).
 
   Section PerObject.
-    Variable obj: Object MvalT StateT.
+    Variable obj: Object MsgT ValT StateT.
 
     (*! Transaction *)
 
-    Definition Responder (rsr: PMsg MvalT StateT) (rs: Msg MvalT) :=
+    Definition Responder (rsr: PMsg MsgT ValT StateT) (rs: Msg MsgT ValT) :=
       exists st mt, In rs (pmsg_outs rsr st mt).
 
     (* A VERY SUBTLE POINT:
      * [rsr] is not a [PMsg] that handles the response,
      * but a [PMsg] that _sends_ the response.
      *)
-    Definition Transaction (rq rsr: PMsg MvalT StateT) (rs: Msg MvalT) :=
+    Definition Transaction (rq rsr: PMsg MsgT ValT StateT) (rs: Msg MsgT ValT) :=
       In rq (obj_pmsgs obj) /\ In rsr (obj_pmsgs obj) /\
       Responder rsr rs /\
       isTrsPair (pmsg_mid rq) (msg_id rs) = true.
 
-    Inductive TransactionInv: PMsg MvalT StateT (* request *) ->
+    Inductive TransactionInv: PMsg MsgT ValT StateT (* request *) ->
                               CondT ->
-                              PMsg MvalT StateT (* response *) -> Prop :=
+                              PMsg MsgT ValT StateT (* response *) -> Prop :=
     | TrsInv: forall rq rsr trsinv,
         postOf rq --> trsinv ->
         trsinv --> pmsg_precond rsr ->
@@ -44,7 +44,7 @@ Section System.
 
     (*! LocallyDisjoint *)
 
-    Definition DisjointTrsInv (rsr: PMsg MvalT StateT) (trsinv: CondT) :=
+    Definition DisjointTrsInv (rsr: PMsg MsgT ValT StateT) (trsinv: CondT) :=
       forall pmsg, In pmsg (obj_pmsgs obj) ->
                    pmsg <> rsr ->
                    (pmsg_precond pmsg) -*- trsinv.
@@ -84,7 +84,7 @@ Section System.
      *)
 
     (* TODO: better definition? *)
-    Definition PDisjointTrsInv (rq rsr: PMsg MvalT StateT) (trsinv: CondT) :=
+    Definition PDisjointTrsInv (rq rsr: PMsg MsgT ValT StateT) (trsinv: CondT) :=
       forall pmsg, In pmsg (obj_pmsgs obj) ->
                    pmsg <> rsr ->
                    (msg_rqrs (pmsg_mid pmsg) = Rq ->
@@ -106,7 +106,7 @@ Section System.
     (* A predicated message is [Immediate] if it handles a request and immediately
      * sends the response of it.
      *)
-    Definition Immediate (rq: PMsg MvalT StateT) :=
+    Definition Immediate (rq: PMsg MsgT ValT StateT) :=
       msg_rqrs (pmsg_mid rq) = Rq /\
       forall st mt, exists rs,
           pmsg_outs rq st mt = rs :: nil /\
@@ -118,7 +118,7 @@ Section System.
      * 3) [rq1] sends a request [rq2] which matches with [rs2], and
      * 4) [rs2] sends a response [rs1] which matches with [rq1].
      *)
-    Definition Forwarding (rq1 rs2: PMsg MvalT StateT) :=
+    Definition Forwarding (rq1 rs2: PMsg MsgT ValT StateT) :=
       msg_rqrs (pmsg_mid rq1) = Rq /\
       msg_rqrs (pmsg_mid rs2) = Rs /\
       (forall st mt, exists rq2,
@@ -132,8 +132,8 @@ Section System.
     (* A predicated message [pmsg] is a unique handler in [pmsgs] if it is
      * the only one handling a certain [MsgId].
      *)
-    Definition UniqueHandler (pmsgs: list (PMsg MvalT StateT))
-               (pmsg: PMsg MvalT StateT) :=
+    Definition UniqueHandler (pmsgs: list (PMsg MsgT ValT StateT))
+               (pmsg: PMsg MsgT ValT StateT) :=
       In pmsg pmsgs /\
       forall pmsg', In pmsg' pmsgs -> (pmsg_mid pmsg) <> (pmsg_mid pmsg').
 
@@ -143,14 +143,14 @@ Section System.
      * object is monotone if they are composed only of [Immediate] or 
      * [Forwarding] messages.
      *)
-    Definition MonotonePMsgs (pmsgs: list (PMsg MvalT StateT)): Prop :=
-      forall (pmsg: PMsg MvalT StateT),
+    Definition MonotonePMsgs (pmsgs: list (PMsg MsgT ValT StateT)): Prop :=
+      forall (pmsg: PMsg MsgT ValT StateT),
         In pmsg pmsgs ->
         (Immediate pmsg \/
-         (exists (rs: PMsg MvalT StateT),
+         (exists (rs: PMsg MsgT ValT StateT),
              In rs pmsgs /\
              Forwarding pmsg rs) \/
-         (exists (rq: PMsg MvalT StateT),
+         (exists (rq: PMsg MsgT ValT StateT),
              In rq pmsgs /\
              Forwarding rq pmsg /\
              UniqueHandler pmsgs pmsg)).
@@ -162,42 +162,42 @@ Section System.
 End System.
 
 Section Facts.
-  Context {MsgT StateT: Type}.
-  Context {MvalT: MsgT -> RqRs -> Type}.
+  Context {MsgT ValT StateT: Type}.
   Hypothesis (msgT_dec : forall m1 m2 : MsgT, {m1 = m2} + {m1 <> m2}).
+  Hypothesis (valT_dec : forall v1 v2 : ValT, {v1 = v2} + {v1 <> v2}).
 
   Theorem sequential_linear:
-    forall sys: System MvalT StateT,
-      SequentialSys msgT_dec sys -> Linear msgT_dec sys.
+    forall sys: System MsgT ValT StateT,
+      SequentialSys msgT_dec valT_dec sys -> Linear msgT_dec valT_dec sys.
   Proof.
   Admitted.
 
   Theorem locally_disjoint_sequential:
-    forall obj: Object MvalT StateT,
-      LocallyDisjoint msgT_dec obj -> SequentialSys msgT_dec (obj :: nil).
+    forall obj: Object MsgT ValT StateT,
+      LocallyDisjoint msgT_dec obj -> SequentialSys msgT_dec valT_dec (obj :: nil).
   Proof.
   Admitted.
 
   Corollary locally_disjoint_linear:
-    forall obj: Object MvalT StateT,
-      LocallyDisjoint msgT_dec obj -> Linear msgT_dec (obj :: nil).
+    forall obj: Object MsgT ValT StateT,
+      LocallyDisjoint msgT_dec obj -> Linear msgT_dec valT_dec (obj :: nil).
   Proof.
     intros; apply sequential_linear, locally_disjoint_sequential; auto.
   Qed.
 
   Theorem linear_sequential_compositional:
-    forall (sys: System MvalT StateT),
+    forall (sys: System MsgT ValT StateT),
       Forall (Monotone msgT_dec) sys ->
-      Forall (fun obj => SequentialSys msgT_dec (obj :: nil)) sys ->
-      Linear msgT_dec sys.
+      Forall (fun obj => SequentialSys msgT_dec valT_dec (obj :: nil)) sys ->
+      Linear msgT_dec valT_dec sys.
   Proof.
   Admitted.
 
   Corollary disjoint_linear:
-    forall (sys: System MvalT StateT),
+    forall (sys: System MsgT ValT StateT),
       Forall (Monotone msgT_dec) sys ->
       Forall (LocallyDisjoint msgT_dec) sys ->
-      Linear msgT_dec sys.
+      Linear msgT_dec valT_dec sys.
   Proof.
     intros; apply linear_sequential_compositional; auto.
     apply Forall_impl with (P:= LocallyDisjoint msgT_dec); auto.
@@ -205,11 +205,11 @@ Section Facts.
   Qed.
 
   Theorem prioritized_interf_linear_compositional:
-    forall (sys: System MvalT StateT),
+    forall (sys: System MsgT ValT StateT),
       Forall (Monotone msgT_dec) sys ->
-      Forall (fun obj => Linear msgT_dec (obj :: nil)) sys ->
+      Forall (fun obj => Linear msgT_dec valT_dec (obj :: nil)) sys ->
       Forall (PInterfering msgT_dec) sys ->
-      Linear msgT_dec sys.
+      Linear msgT_dec valT_dec sys.
   Proof.
   Admitted.
 
